project02/MessageType.v.dfy
@@ -3,6 +3,6 @@ module MessageType {
 /*{*/
     | Get(key: int, value: int)
     | Put(key: int, value: int)
-    | KeyValue(key: int, value: int)
+    | KeyValue(key: int, value: int, idx: nat)
 /*}*/
 }
